@prefix rdf: <http://www.w3.org/1999/02/22-rdf-syntax-ns#> .
@prefix foaf: <http://xmlns.com/foaf/0.1/> .
@prefix madsrdf: <http://www.loc.gov/mads/rdf/v1#> .
@prefix owl: <http://www.w3.org/2002/07/owl#> .
@prefix rdfs: <http://www.w3.org/2000/01/rdf-schema#> .
@prefix xsd: <http://www.w3.org/2001/XMLSchema#> .
@prefix : <http://www.loc.gov/standards/mads/rdf/v1.rdf#> .

madsrdf:Address
    a owl:Class ;
    rdfs:label "Address"@en .

madsrdf:Affiliation
    a owl:Class ;
    rdfs:comment """A resource that describes an individual's affiliation with an
      organization or group, such as the nature of the affiliation and the active
      dates."""@en ;
    rdfs:label "Affiliation"@en .

madsrdf:Area
    a owl:Class ;
    rdfs:comment """Describes a resource whose
      label is a non-jurisdictional geographic entity."""^^xsd:string ;
    rdfs:label "Area Type"@en ;
    rdfs:subClassOf madsrdf:Geographic .

madsrdf:Authority
    a owl:Class ;
    rdfs:comment """A concept with a controlled
      label."""^^xsd:string ;
    rdfs:label "Authority"@en ;
    rdfs:subClassOf owl:Thing, <http://www.w3.org/2004/02/skos/core#Concept> ;
    owl:disjointWith madsrdf:DeprecatedAuthority, madsrdf:MADSCollection, madsrdf:MADSScheme, madsrdf:Variant .

madsrdf:City
    a owl:Class ;
    rdfs:comment """Describes a resource whose
      label is an inhabited place incorporated as a city, town, etc."""^^xsd:string ;
    rdfs:label "City Type"@en ;
    rdfs:subClassOf madsrdf:Geographic .

madsrdf:CitySection
    a owl:Class ;
    rdfs:comment """Describes a resource whose
      label is a smaller unit within a populated place, e.g., a neighborhood, park, or
      street."""^^xsd:string ;
    rdfs:label "City Section Type"@en ;
    rdfs:subClassOf madsrdf:Geographic .

madsrdf:ComplexSubject
    a owl:Class ;
    rdfs:comment """The label of a madsrdf:ComplexSubject is the concatenation of labels
      from two or more madsrdf:SimpleType descriptions, except that the combination of
      madsrdf:SimpleType labels for the madsrdf:ComplexSubject does not meet the conditions to be
      the label of a madsrdf:NameTitle resource or madsrdf:HierarchicalGeographic
      resource."""@en ;
    rdfs:label "Complex Subject Type"@en ;
    rdfs:subClassOf madsrdf:ComplexType .

madsrdf:ComplexType
    a owl:Class ;
    rdfs:comment """madsrdf:ComplexType is a resource whose label is the concatenation
      of labels from two or more Authority descriptions or two or more Variant descriptions or some
      combination of Authority and Variant descriptions, each of a
      madsrdf:SimpleType."""@en ;
    rdfs:label "Complex Type"@en ;
    rdfs:subClassOf madsrdf:MADSType ;
    owl:disjointUnionOf (madsrdf:HierarchicalGeographic
        madsrdf:ComplexSubject
        madsrdf:NameTitle
    ) ;
    owl:disjointWith madsrdf:SimpleType ;
    owl:equivalentClass [
        a owl:Restriction ;
        owl:cardinality "1"^^xsd:nonNegativeInteger ;
        owl:onProperty madsrdf:componentList
    ] .

madsrdf:ConferenceName
    a owl:Class ;
    rdfs:comment """Describes a resource whose
      label represents a conference name."""^^xsd:string ;
    rdfs:label "Conference Name Type"@en ;
    rdfs:subClassOf madsrdf:Name .

madsrdf:Continent
    a owl:Class ;
    rdfs:comment """Describes a resource whose
      label is one of seven large landmasses on Earth. These are: Asia, Africa, Europe, North
      America, South America, Australia, and Antarctica."""^^xsd:string ;
    rdfs:label "Continent Type"@en ;
    rdfs:subClassOf madsrdf:Geographic .

madsrdf:CorporateName
    a owl:Class ;
    rdfs:comment """Describes a resource whose
      label is the name of a corporate entity, which may include political or ecclesiastical
      entities."""^^xsd:string ;
    rdfs:label "Corporate Name Type"@en ;
    rdfs:subClassOf madsrdf:Name .

madsrdf:Country
    a owl:Class ;
    rdfs:comment """Describes a resource whose
      label is a country, i.e. a political entity considered a country. """^^xsd:string ;
    rdfs:label "Country Type"@en ;
    rdfs:subClassOf madsrdf:Geographic .

madsrdf:County
    a owl:Class ;
    rdfs:comment """Describes a resource whose
      label is the largest local administrative unit, e.g. Warwickshire, in a country, e.g.
      England."""^^xsd:string ;
    rdfs:label "County Type"@en ;
    rdfs:subClassOf madsrdf:Geographic .

madsrdf:DateNameElement
    a owl:Class ;
    rdfs:label """Date Name
      Element"""^^xsd:string ;
    rdfs:subClassOf madsrdf:NameElement .

madsrdf:DeprecatedAuthority
    a owl:Class ;
    rdfs:comment """A former
      Authority."""^^xsd:string ;
    rdfs:label """Deprecated
      Authority"""^^xsd:string ;
    rdfs:subClassOf owl:Thing ;
    owl:disjointWith madsrdf:Authority, madsrdf:MADSCollection, madsrdf:MADSScheme .

madsrdf:Element
    a owl:Class ;
    rdfs:comment """madsrdf:Element types
      describe the various parts of labels."""^^xsd:string ;
    rdfs:label "Element"@en ;
    owl:equivalentClass [
        a owl:Restriction ;
        owl:cardinality "1"^^xsd:nonNegativeInteger ;
        owl:onProperty madsrdf:elementValue
    ] .

madsrdf:ExtraterrestrialArea
    a owl:Class ;
    rdfs:comment """Describes a resource whose
      label is any extraterrestrial entity or space, including a solar system, a galaxy, a star
      system, and a planet, including a geographic feature of an individual planet."""^^xsd:string ;
    rdfs:label "Extraterrestrial Area Type"@en ;
    rdfs:subClassOf madsrdf:Geographic .

madsrdf:FamilyName
    a owl:Class ;
    rdfs:comment """Describes a resource whose
      label represents a family name."""^^xsd:string ;
    rdfs:label "Family Name Type"@en ;
    rdfs:subClassOf madsrdf:Name .

madsrdf:FamilyNameElement
    a owl:Class ;
    rdfs:label """Family Name
      Element"""^^xsd:string ;
    rdfs:subClassOf madsrdf:NameElement .

madsrdf:FullNameElement
    a owl:Class ;
    rdfs:label "Fullname Element"^^xsd:string ;
    rdfs:subClassOf madsrdf:NameElement .

madsrdf:GenreForm
    a owl:Class ;
    rdfs:comment """Describes a resource whose label is a genre or form term. Genre
      terms for textual materials designate specific kinds of materials distinguished by the style
      or technique of their intellectual contents; for example, biographies, catechisms, essays,
      hymns, or reviews. Form terms designate historically and functionally specific kinds of
      materials as distinguished by an examination of their physical character, characteristics of
      their intellectual content, or the order of information within them; for example, daybooks,
      diaries, directories, journals, memoranda, questionnaires, syllabi, or time sheets. In the
      context of graphic materials, genre headings denote categories of material distinguished by
      vantage point, intended purpose, characteristics of the creator, publication status, or method
      of representation."""@en ;
    rdfs:label "Genre/Form Type"@en ;
    rdfs:subClassOf madsrdf:SimpleType .

madsrdf:GenreFormElement
    a owl:Class ;
    rdfs:label "Genre/Form Element"@en ;
    rdfs:subClassOf madsrdf:Element .

madsrdf:Geographic
    a owl:Class ;
    rdfs:comment """Describes a resource whose label represents a geographic place or
      feature, especially when a more precise geographic determination (City, Country, Region, etc.)
      cannot be made."""@en ;
    rdfs:label "Geographic Authority"@en ;
    rdfs:subClassOf madsrdf:SimpleType .

madsrdf:GeographicElement
    a owl:Class ;
    rdfs:label "Geographic Element"@en ;
    rdfs:subClassOf madsrdf:Element .

madsrdf:GivenNameElement
    a owl:Class ;
    rdfs:label """Given Name
      Element"""^^xsd:string ;
    rdfs:subClassOf madsrdf:NameElement .

madsrdf:HierarchicalGeographic
    a owl:Class ;
    rdfs:comment """A madsrdf:HierarchicalGeographic indicates that its label is the
      concatenation of labels from a sequence of madsrdf:Geographic types taken from one of the
      madsrdf:Geographic sub-classes such as madsrdf:City, madsrdf:Country, madsrdf:State,
      madsrdf:Region, madsrdf:Area, etc. The madsrdf:Geographic resources that constitute the
      madsrdf:HierarchicalGeographic should have a broader to narrower hierarchical relationship
      between them."""@en ;
    rdfs:label "Hierarchical Geographic Type"@en ;
    rdfs:subClassOf madsrdf:ComplexType .

madsrdf:Identifier
    a owl:Class ;
    rdfs:comment """A madsrdf:Identifier
      resource describes an identifier by associating the identifier value with its type. To be used
      to record identifiers for a resource in the absence of URIs."""^^xsd:string ;
    rdfs:label "Other Identifier"^^xsd:string .

madsrdf:Island
    a owl:Class ;
    rdfs:comment """Describes a resource whose
      label is a tract of land surrounded by water and smaller than a continent but is not itself a
      separate country. """^^xsd:string ;
    rdfs:label "Island Type"@en ;
    rdfs:subClassOf madsrdf:Geographic .

madsrdf:Language
    a owl:Class ;
    rdfs:comment """Describes a resource whose label represents a
      language."""@en ;
    rdfs:label "Language Type"@en ;
    rdfs:subClassOf madsrdf:SimpleType ;
    owl:equivalentClass <http://purl.org/dc/terms/LinguisticSystem> .

madsrdf:LanguageElement
    a owl:Class ;
    rdfs:label "Language Element"^^xsd:string ;
    rdfs:subClassOf madsrdf:Element .

madsrdf:MADSCollection
    a owl:Class ;
    rdfs:comment """A madsrdf:Collection is an
      organizational unit, members of which will have some form of intellectually unifying theme but
      not to the extent that it defines an independent knowledge organization system. It aggregates
      madsrdf:Authority descriptions or other madsrdf:MADSCollection resources."""^^xsd:string ;
    rdfs:label "MADS Collection"^^xsd:string ;
    rdfs:subClassOf <http://www.w3.org/2004/02/skos/core#Collection> ;
    owl:disjointWith madsrdf:Authority, madsrdf:MADSScheme, madsrdf:Variant .

madsrdf:MADSScheme
    a owl:Class ;
    rdfs:comment """MADS Scheme is an organizational unit that describes a knowledge
      organization system. It aggregates madsrdf:Authority descriptions and/or
      madsrdf:MADSCollection resources included in the knowledge organization system. Including a
      madsrdf:MADSCollection within a madsrdf:MADSScheme should be done with care; when a
      madsrdf:MADSCollection is part of a madsrdf:MADSScheme, then any madsrdf:Authority within that
      madsrdf:MADSCollection is effectively also in the madsrdf:MADSScheme."""@en ;
    rdfs:label "MADS Scheme"@en ;
    rdfs:subClassOf <http://www.w3.org/2004/02/skos/core#ConceptScheme> ;
    owl:disjointWith madsrdf:Authority, madsrdf:MADSCollection, madsrdf:Variant .

madsrdf:MADSType
    a owl:Class ;
    rdfs:label "MADS Type"^^xsd:string ;
    owl:disjointWith madsrdf:MADSCollection, madsrdf:MADSScheme .

madsrdf:MainTitleElement
    a owl:Class ;
    rdfs:label """Main Title
      Element"""^^xsd:string ;
    rdfs:subClassOf madsrdf:TitleElement .

madsrdf:Name
    a owl:Class ;
    rdfs:comment """Describes a resource whose label represents a name, especially when
      a more precise Name type (madsrdf:ConferenceName, masdrdf:FamilyName, etc.) cannot be
      identified."""@en ;
    rdfs:label "Name Type"@en ;
    rdfs:subClassOf madsrdf:SimpleType .

madsrdf:NameElement
    a owl:Class ;
    rdfs:label "Name Element"@en ;
    rdfs:subClassOf madsrdf:Element .

madsrdf:NameTitle
    a owl:Class ;
    rdfs:comment """The label of a madsrdf:NameTitle resource is the concatenation of a
      label of a madsrdf:Name description and the label of a madsrdf:Title description. Both
      description types (madsrdf:Name and madsrdf:Title) are of madsrdf:SimpleType
      types."""@en ;
    rdfs:label "Name/Title Type"@en ;
    rdfs:subClassOf madsrdf:ComplexType .

madsrdf:NonSortElement
    a owl:Class ;
    rdfs:label "Non-sort Element"^^xsd:string ;
    rdfs:subClassOf madsrdf:TitleElement .

madsrdf:Occupation
    a owl:Class ;
    rdfs:comment """Describes a resource whose
      label represents an occcupation."""^^xsd:string ;
    rdfs:label "Occupation Type"@en ;
    rdfs:subClassOf madsrdf:SimpleType .

madsrdf:PartNameElement
    a owl:Class ;
    rdfs:label """Part Name
      Element"""^^xsd:string ;
    rdfs:subClassOf madsrdf:TitleElement .

madsrdf:PartNumberElement
    a owl:Class ;
    rdfs:label """Part Number
      Element"""^^xsd:string ;
    rdfs:subClassOf madsrdf:TitleElement .

madsrdf:PersonalName
    a owl:Class ;
    rdfs:comment """Describes a resource whose
      label represents a personal name."""^^xsd:string ;
    rdfs:label "Personal Name Type"@en ;
    rdfs:subClassOf madsrdf:Name .

madsrdf:Province
    a owl:Class ;
    rdfs:comment """Describes a resource whose
      label is a first order political division, e.g. Ontario, within a country, e.g. Canada. """^^xsd:string ;
    rdfs:label "Province Type"@en ;
    rdfs:subClassOf madsrdf:Geographic .

madsrdf:RWO
    a owl:Class ;
    rdfs:comment """A madsrdf:RWO is an
      abstract entity and identifies a Real World Object (RWO) identified by the label of a
      madsrdf:Authority or madsrdf:DeprecatedAuthority."""^^xsd:string ;
    rdfs:label """Real World
      Object"""^^xsd:string ;
    rdfs:subClassOf owl:Thing .

madsrdf:Region
    a owl:Class ;
    rdfs:comment """Describes a resource whose
      label is an area that has the status of a jurisdiction, usually incorporating more than one
      first level jurisdiction. """^^xsd:string ;
    rdfs:label "Region Type"@en ;
    rdfs:subClassOf madsrdf:Geographic .

madsrdf:SimpleType
    a owl:Class ;
    rdfs:comment """madsrdf:SimpleType is a resource with a label constituting a single
      word or phrase."""@en ;
    rdfs:label "Simple Type"@en ;
    rdfs:subClassOf madsrdf:MADSType .

madsrdf:Source
    a owl:Class ;
    rdfs:comment """A resource that represents
      the source of information about another resource. madsrdf:Source is a type of
      citation."""^^xsd:string ;
    rdfs:label "Source"^^xsd:string .

madsrdf:State
    a owl:Class ;
    rdfs:comment """Describes a resource whose
      label is a first order political division, e.g. Montana, within a country, e.g.
      U.S."""^^xsd:string ;
    rdfs:label "State Type"@en ;
    rdfs:subClassOf madsrdf:Geographic .

madsrdf:SubTitleElement
    a owl:Class ;
    rdfs:label "Subtitle Element"^^xsd:string ;
    rdfs:subClassOf madsrdf:TitleElement .

madsrdf:Temporal
    a owl:Class ;
    rdfs:comment """Describes a resource whose
      label represents a time-based notion."""^^xsd:string ;
    rdfs:label "Temporal Type"@en ;
    rdfs:subClassOf madsrdf:SimpleType .

madsrdf:TemporalElement
    a owl:Class ;
    rdfs:label "Temporal Element"^^xsd:string ;
    rdfs:subClassOf madsrdf:Element .

madsrdf:TermsOfAddressNameElement
    a owl:Class ;
    rdfs:label """Terms of Address
      Element"""^^xsd:string ;
    rdfs:subClassOf madsrdf:NameElement .

madsrdf:Territory
    a owl:Class ;
    rdfs:comment """Describes a resource whose
      label is a geographical area belonging to or under the jurisdiction of a governmental
      authority. """^^xsd:string ;
    rdfs:label "Territory Type"@en ;
    rdfs:subClassOf madsrdf:Geographic .

madsrdf:Title
    a owl:Class ;
    rdfs:comment """Describes a resource whose
      label represents a title."""^^xsd:string ;
    rdfs:label "Title Type"@en ;
    rdfs:subClassOf madsrdf:SimpleType .

madsrdf:TitleElement
    a owl:Class ;
    rdfs:label "Title Element"@en ;
    rdfs:subClassOf madsrdf:Element .

madsrdf:Topic
    a owl:Class ;
    rdfs:comment """Describes a resource whose
      label represents a topic."""^^xsd:string ;
    rdfs:label "Topic Type"@en ;
    rdfs:subClassOf madsrdf:SimpleType .

madsrdf:TopicElement
    a owl:Class ;
    rdfs:label "Topic Element"@en ;
    rdfs:subClassOf madsrdf:Element .

madsrdf:Variant
    a owl:Class ;
    rdfs:comment """A resource whose label is the alternate form of an Authority or
      Deprecated Authority."""@en ;
    rdfs:label "Variant"@en ;
    rdfs:subClassOf owl:Thing, <http://www.w3.org/2008/05/skos-xl#Label> ;
    owl:disjointWith madsrdf:Authority, madsrdf:MADSCollection, madsrdf:MADSScheme .

madsrdf:activityEndDate
    a rdf:Property, owl:DatatypeProperty ;
    rdfs:comment """Latest date in a period of activity.
    """^^xsd:string ;
    rdfs:domain madsrdf:RWO ;
    rdfs:label "Activity End"^^xsd:string .

madsrdf:activityStartDate
    a rdf:Property, owl:DatatypeProperty ;
    rdfs:comment """Earliest date in a period of activity.
    """^^xsd:string ;
    rdfs:domain madsrdf:RWO ;
    rdfs:label "Activity Start"^^xsd:string .

madsrdf:adminMetadata
    a rdf:Property, owl:ObjectProperty ;
    rdfs:comment """This relates an Authority or Variant to its administrative metadata,
      which is, minimimally, a Class defined outside of the MADS/RDF namespace. The RecordInfo Class
      from the RecordInfo ontology is recommended."""@en ;
    rdfs:domain [
        a owl:Class ;
        owl:unionOf (madsrdf:Authority
            madsrdf:DeprecatedAuthority
            madsrdf:Variant
        )
    ] ;
    rdfs:label "Administrative Metadata"@en .

madsrdf:affiliationEnd
    a rdf:Property, owl:DatatypeProperty ;
    rdfs:comment """The date an individual
      ceased to be affiliated with an organization."""^^xsd:string ;
    rdfs:domain madsrdf:Affiliation ;
    rdfs:label """Affiliation
      Ended"""^^xsd:string ;
    rdfs:range xsd:date .

madsrdf:affiliationStart
    a rdf:Property, owl:DatatypeProperty ;
    rdfs:comment """The date an individual
      established an affiliation with an organization."""^^xsd:string ;
    rdfs:domain madsrdf:Affiliation ;
    rdfs:label """Affiliation
      Started"""^^xsd:string ;
    rdfs:range xsd:date .

madsrdf:associatedLanguage
    a rdf:Property, owl:ObjectProperty ;
    rdfs:comment """Language that a person,
      organization, or family uses for publication, communication, etc., or in which a work is
      expressed. """^^xsd:string ;
    rdfs:domain madsrdf:RWO ;
    rdfs:label """Associated
      Language"""^^xsd:string ;
    rdfs:range madsrdf:Language .

madsrdf:associatedLocale
    a rdf:Property, owl:ObjectProperty ;
    rdfs:comment """A town, city, province,
      state, and/or country associated with persons, corporate bodies, families, works, and
      expressions."""^^xsd:string ;
    rdfs:domain madsrdf:RWO ;
    rdfs:label "Associated Locale"^^xsd:string ;
    rdfs:range madsrdf:Geographic .

madsrdf:authoritativeLabel
    a rdf:Property, owl:AnnotationProperty ;
    rdfs:comment """A lexical string representing a controlled, curated label for the
      Authority."""@en ;
    rdfs:domain madsrdf:Authority ;
    rdfs:label "Authoritative Label"@en ;
    rdfs:subPropertyOf rdfs:label, <http://www.w3.org/2004/02/skos/core#prefLabel> .

madsrdf:birthDate
    a rdf:Property, owl:DatatypeProperty ;
    rdfs:comment """The year a person was born.
      Date of birth may also include the month and day of the person’s birth. (RDA
      9.3.2.1)"""^^xsd:string ;
    rdfs:domain madsrdf:RWO ;
    rdfs:label "Birth Date"^^xsd:string .

madsrdf:birthPlace
    a rdf:Property, owl:ObjectProperty ;
    rdfs:comment """The town, city, province,
      state, and/or country in which a person was born."""^^xsd:string ;
    rdfs:domain madsrdf:RWO ;
    rdfs:label "Place of Birth"^^xsd:string ;
    rdfs:range madsrdf:Geographic .

madsrdf:changeNote
    a rdf:Property, owl:AnnotationProperty ;
    rdfs:comment """A note detailing a modification to an Authority or
      Variant."""@en ;
    rdfs:label "Change Note"@en ;
    rdfs:subPropertyOf madsrdf:note ;
    owl:equivalentProperty <http://www.w3.org/2004/02/skos/core#changeNote> .

madsrdf:citationNote
    a rdf:Property, owl:AnnotationProperty ;
    rdfs:comment """A note about how the madsrdf:Source relates to the resource about
      which the madsrdf:Source is the information source."""@en ;
    rdfs:domain madsrdf:Source ;
    rdfs:label "Citation Note"@en .

madsrdf:citationSource
    a rdf:Property, owl:AnnotationProperty ;
    rdfs:comment "The cited resource."@en ;
    rdfs:domain madsrdf:Source ;
    rdfs:label "Citation Source"@en .

madsrdf:citationStatus
    a rdf:Property, owl:DatatypeProperty ;
    rdfs:comment """Should use a standard term - such as 'found' or 'not found' - to
      indicate whether the cited resource yielded information about the resource related to the
      madsrdf:Source."""@en ;
    rdfs:domain madsrdf:Source ;
    rdfs:label "Citation Status"@en ;
    rdfs:range xsd:string .

madsrdf:city
    a rdf:Property, owl:AnnotationProperty ;
    rdfs:comment "The city component of an address."@en ;
    rdfs:domain madsrdf:Address ;
    rdfs:label "City"@en .

madsrdf:classification
    a rdf:Property, owl:AnnotationProperty ;
    rdfs:comment """The classification code associated with a
      madsrdf:Authority."""@en ;
    rdfs:domain madsrdf:Authority ;
    rdfs:label "Classification"@en ;
    rdfs:subPropertyOf <http://www.w3.org/2004/02/skos/core#semanticRelation> .

madsrdf:code
    a rdf:Property, owl:DatatypeProperty ;
    rdfs:comment """A code is a string of
      characters associated with a the authoritative or deprecated label. It may record an
      historical notation once used to uniquely identify a concept."""^^xsd:string ;
    rdfs:domain [
        a owl:Class ;
        owl:unionOf (madsrdf:Authority
            madsrdf:DeprecatedAuthority
        )
    ] ;
    rdfs:label "Code"^^xsd:string ;
    rdfs:subPropertyOf <http://www.w3.org/2004/02/skos/core#notation> .

madsrdf:componentList
    a rdf:Property, owl:ObjectProperty ;
    rdfs:comment """madsrdf:componentList
      organizes the madsrdf:SimpleType resources whose labels are represented in the label of the
      associated madsrdf:ComplexType resource."""^^xsd:string ;
    rdfs:domain madsrdf:ComplexType ;
    rdfs:label "Component List"^^xsd:string ;
    rdfs:range [
        a owl:Class ;
        owl:unionOf (rdf:List
            rdf:Seq
        )
    ] .

madsrdf:country
    a rdf:Property, owl:AnnotationProperty ;
    rdfs:comment """Country associated with an
      address."""^^xsd:string ;
    rdfs:domain madsrdf:Address ;
    rdfs:label "Country"^^xsd:string .

madsrdf:creationDateEnd
    a rdf:Property, owl:DatatypeProperty ;
    rdfs:comment "Ending date of the date range for which the beginning date is recorded in madsrdf:creationDateStart."^^xsd:string ;
    rdfs:label ""^^xsd:string .

madsrdf:creationDateStart
    a rdf:Property, owl:DatatypeProperty ;
    rdfs:comment "For a work, earliest date (normally the year) associated with a work; that date may be the date the work was created or first published or released. For an expression, the earliest date (normally the year) associated with an expression; that date may be the date of the earliest known manifestation of that expression. In both cases the date may be the starting date of a range or a single date."^^xsd:string ;
    rdfs:label "Work begun"^^xsd:string .

madsrdf:deathDate
    a rdf:Property, owl:DatatypeProperty ;
    rdfs:comment """The year a person died.
      Date of death may also include the month and day of the person’s death. (RDA
      9.3.3.1)"""^^xsd:string ;
    rdfs:domain madsrdf:RWO ;
    rdfs:label "Death Date"^^xsd:string .

madsrdf:deathPlace
    a rdf:Property, owl:ObjectProperty ;
    rdfs:comment """The town, city, province,
      state, and/or country in which a person died."""^^xsd:string ;
    rdfs:domain madsrdf:RWO ;
    rdfs:label "Place of Death"^^xsd:string ;
    rdfs:range madsrdf:Geographic .

madsrdf:definitionNote
    a rdf:Property, owl:AnnotationProperty ;
    rdfs:comment """An explanation of the meaning of an Authority, DeprecatedAuthority,
      or Variant description."""@en ;
    rdfs:label "Definition Note"@en ;
    rdfs:subPropertyOf madsrdf:note ;
    owl:equivalentProperty <http://www.w3.org/2004/02/skos/core#definition> .

madsrdf:deletionNote
    a rdf:Property, owl:AnnotationProperty ;
    rdfs:comment """A note pertaining to the
      deletion of a resource."""^^xsd:string ;
    rdfs:label "Deletion Note"^^xsd:string ;
    rdfs:subPropertyOf madsrdf:changeNote .

madsrdf:deprecatedLabel
    a rdf:Property, owl:AnnotationProperty ;
    rdfs:comment """A label once considered
      authoritative (controlled and curated) but which is no longer."""^^xsd:string ;
    rdfs:domain madsrdf:DeprecatedAuthority ;
    rdfs:label "Deprecated Label"^^xsd:string ;
    rdfs:subPropertyOf rdfs:label, <http://www.w3.org/2004/02/skos/core#hiddenLabel> .

madsrdf:editorialNote
    a rdf:Property, owl:AnnotationProperty ;
    rdfs:comment """A note pertaining to the
      management of the label associated with the resource."""^^xsd:string ;
    rdfs:label "Editorial Note"^^xsd:string ;
    rdfs:subPropertyOf madsrdf:note ;
    owl:equivalentProperty <http://www.w3.org/2004/02/skos/core#editorialNote> .

madsrdf:elementList
    a rdf:Property, owl:ObjectProperty ;
    rdfs:comment """The madsrdf:elementList property is used to organize the various
      parts of labels."""@en ;
    rdfs:label "Element List"^^xsd:string ;
    rdfs:range [
        a owl:Class ;
        owl:unionOf (rdf:List
            rdf:Seq
        )
    ] .

madsrdf:elementValue
    a rdf:Property, owl:DatatypeProperty ;
    rdfs:domain madsrdf:Element ;
    rdfs:label "Element Value"^^xsd:string ;
    rdfs:range xsd:string .

madsrdf:email
    a rdf:Property, owl:DatatypeProperty ;
    rdfs:domain madsrdf:Affiliation ;
    rdfs:label "Email"^^xsd:string .

madsrdf:entityDescriptor
    a rdf:Property, owl:DatatypeProperty ;
    rdfs:comment """Any attribute that serves
      to characterize a person, family or corporate body or that may be needed for differentiation
      from other persons. families or corporate bodies and for which separate content designation is
      not already defined.Or """^^xsd:string ;
    rdfs:domain madsrdf:RWO ;
    rdfs:label """Entity
      Descriptor"""^^xsd:string .

madsrdf:establishDate
    a rdf:Property, owl:DatatypeProperty ;
    rdfs:comment """The year a corporate body was established. Date of establishment may also include the month and day of the corporate body’s establishment.
    """^^xsd:string ;
    rdfs:domain madsrdf:RWO ;
    rdfs:label "Established"^^xsd:string .

madsrdf:exampleNote
    a rdf:Property, owl:AnnotationProperty ;
    rdfs:comment """A example of how the
      resource might be used."""^^xsd:string ;
    rdfs:label "Example Note"^^xsd:string ;
    rdfs:subPropertyOf madsrdf:note ;
    owl:equivalentProperty <http://www.w3.org/2004/02/skos/core#example> .

madsrdf:extendedAddress
    a rdf:Property, owl:DatatypeProperty ;
    rdfs:comment """The second address line, if
      needed."""^^xsd:string ;
    rdfs:domain madsrdf:Address ;
    rdfs:label "Extended Address"^^xsd:string .

madsrdf:extension
    a rdf:Property, owl:ObjectProperty ;
    rdfs:label "Extension"^^xsd:string .

madsrdf:fax
    a rdf:Property, owl:DatatypeProperty ;
    rdfs:comment "Fax number"^^xsd:string ;
    rdfs:domain madsrdf:Affiliation ;
    rdfs:label "Fax"^^xsd:string .

madsrdf:fieldOfActivity
    a rdf:Property, owl:ObjectProperty ;
    rdfs:comment """The field of activity
      associated with an individual."""^^xsd:string ;
    rdfs:domain madsrdf:RWO ;
    rdfs:label """Field of
      Activity"""^^xsd:string .

madsrdf:fullerName
    a rdf:Property, owl:ObjectProperty ;
    rdfs:comment """Full form of name needed to
      distinguish a person from another person with the same preferred name."""^^xsd:string ;
    rdfs:label "Fuller Name"^^xsd:string ;
    rdfs:range madsrdf:PersonalName .

madsrdf:gender
    a rdf:Property, owl:DataTypeProperty ;
    rdfs:comment """The gender with which a
      person identifies. """^^xsd:string ;
    rdfs:domain madsrdf:RWO ;
    rdfs:label "Gender"^^xsd:string .

madsrdf:hasAbbreviationVariant
    a rdf:Property, owl:ObjectProperty ;
    rdfs:label """Has Abbreviation
      Variant"""^^xsd:string ;
    rdfs:subPropertyOf madsrdf:hasVariant .

madsrdf:hasAcronymVariant
    a rdf:Property, owl:ObjectProperty ;
    rdfs:label """Has Acronym
      Variant"""^^xsd:string ;
    rdfs:subPropertyOf madsrdf:hasVariant .

madsrdf:hasAffiliation
    a rdf:Property, owl:ObjectProperty ;
    rdfs:comment """Property to associate an
      individual, such as a foaf:Agent, to a group or organization with which an individual is or
      has been affiliated."""^^xsd:string ;
    rdfs:domain madsrdf:RWO ;
    rdfs:label "Has Affiliation"^^xsd:string ;
    rdfs:range madsrdf:Affiliation .

madsrdf:hasAffiliationAddress
    a rdf:Property, owl:ObjectProperty ;
    rdfs:comment """The address of the group or
      organization with which an individual is associated."""^^xsd:string ;
    rdfs:domain madsrdf:Affiliation ;
    rdfs:label """Has Affiliation
      Address"""^^xsd:string ;
    rdfs:range madsrdf:Address .

madsrdf:hasBroaderAuthority
    a rdf:Property, owl:ObjectProperty ;
    rdfs:label """Has Broader
      Authority"""^^xsd:string ;
    rdfs:subPropertyOf madsrdf:hasRelatedAuthority, <http://www.w3.org/2004/02/skos/core#broader> ;
    owl:inverseOf madsrdf:hasNarrowerAuthority .

madsrdf:hasBroaderExternalAuthority
    a rdf:Property, owl:ObjectProperty ;
    rdfs:comment """Creates a direct
      relationship between an Authority and a more broadly defined Authority from a different MADS
      Scheme."""^^xsd:string ;
    rdfs:label """Has Broader External
      Authority"""^^xsd:string ;
    rdfs:subPropertyOf madsrdf:hasBroaderAuthority, <http://www.w3.org/2004/02/skos/core#broadMatch> .

madsrdf:hasChararacteristic
    a rdf:Property, owl:ObjectProperty ;
    rdfs:comment """A term that specifies a characteristic that differentiates a work or expression from another one.
    """^^xsd:string ;
    rdfs:label "Other characteristic"^^xsd:string .

madsrdf:hasCloseExternalAuthority
    a rdf:Property, owl:ObjectProperty, owl:SymmetricProperty ;
    rdfs:comment """Records a relationship
      between an Authority and one that is closely related from a different MADS
      Scheme."""^^xsd:string ;
    rdfs:label """Has Close External
      Authority"""^^xsd:string ;
    rdfs:subPropertyOf madsrdf:hasRelatedAuthority, <http://www.w3.org/2004/02/skos/core#closeMatch> .

madsrdf:hasCorporateParentAuthority
    a rdf:Property, owl:ObjectProperty ;
    rdfs:comment """Establishes a relationship
      between a CorporateName Authority and one of the same that is more broadly
      defined."""^^xsd:string ;
    rdfs:domain madsrdf:CorporateName ;
    rdfs:label """Has Parent
      Organization"""^^xsd:string ;
    rdfs:range madsrdf:CorporateName ;
    rdfs:subPropertyOf madsrdf:hasRelatedAuthority .

madsrdf:hasCorporateSubsidiaryAuthority
    a rdf:Property, owl:ObjectProperty ;
    rdfs:comment """Establishes a relationship
      between a CorporateName Authority and one of the same that is more narrowly
      defined."""^^xsd:string ;
    rdfs:domain madsrdf:CorporateName ;
    rdfs:label """Is Parent Organization
      Of"""^^xsd:string ;
    rdfs:range madsrdf:CorporateName ;
    rdfs:subPropertyOf madsrdf:hasRelatedAuthority ;
    owl:inverseOf madsrdf:hasCorporateParentAuthority .

madsrdf:hasEarlierEstablishedForm
    a rdf:Property, owl:ObjectProperty ;
    rdfs:comment """Used to reference a resource that was an earlier form. This is
      Related type='earlier' in MADS XML."""@en ;
    rdfs:label """Has Earlier Established
      Form"""^^xsd:string ;
    rdfs:subPropertyOf madsrdf:see ;
    owl:inverseOf madsrdf:hasLaterEstablishedForm .

madsrdf:hasExactExternalAuthority
    a rdf:Property, owl:ObjectProperty, owl:SymmetricProperty, owl:TransitiveProperty ;
    rdfs:comment """Records a relationship
      between an Authority and one to which it matches exactly but from a different MADS
      Scheme."""^^xsd:string ;
    rdfs:label """Has Exact External
      Authority"""^^xsd:string ;
    rdfs:subPropertyOf madsrdf:hasCloseExternalAuthority, <http://www.w3.org/2004/02/skos/core#exactMatch> .

madsrdf:hasExpansionVariant
    a rdf:Property, owl:ObjectProperty ;
    rdfs:label """Has Expansion
      Variant"""^^xsd:string ;
    rdfs:subPropertyOf madsrdf:hasVariant .

madsrdf:hasHiddenVariant
    a rdf:Property, owl:ObjectProperty ;
    rdfs:comment """Use for variants that are searchable, but not necessarily for
      display."""@en ;
    rdfs:domain madsrdf:Authority ;
    rdfs:label "Has Hidden Variant"@en ;
    rdfs:range madsrdf:Variant ;
    rdfs:subPropertyOf <http://www.w3.org/2008/05/skos-xl#hiddenLabel> .

madsrdf:hasIdentifier
    a rdf:Property, owl:ObjectProperty ;
    rdfs:comment """Associates a resource with
      a madsrdf:Identifier."""^^xsd:string ;
    rdfs:label "Has Identifier"^^xsd:string ;
    rdfs:range madsrdf:Identifier .

madsrdf:hasLaterEstablishedForm
    a rdf:Property, owl:ObjectProperty ;
    rdfs:comment """Use to reference the later form of a resource. This is Related
      type='later' in MADS XML."""@en ;
    rdfs:label """Has Later Established
      Form"""^^xsd:string ;
    rdfs:subPropertyOf madsrdf:see ;
    owl:inverseOf madsrdf:hasEarlierEstablishedForm .

madsrdf:hasMADSCollectionMember
    a rdf:Property, owl:ObjectProperty ;
    rdfs:comment """Associates an Authority or other Collection with a
      madsrdf:MADSCollection."""@en ;
    rdfs:domain madsrdf:MADSCollection ;
    rdfs:label "Has MADSCollection Member"@en ;
    rdfs:range [
        a owl:Class ;
        owl:unionOf (madsrdf:Authority
            madsrdf:MADSCollection
        )
    ] ;
    rdfs:subPropertyOf <http://www.w3.org/2004/02/skos/core#member> ;
    owl:inverseOf madsrdf:isMemberOfMADSCollection .

madsrdf:hasMADSSchemeMember
    a rdf:Property, owl:ObjectProperty ;
    rdfs:comment """Associates an Authority or Collection with a
      madsrdf:MADSScheme."""@en ;
    rdfs:domain madsrdf:MADSScheme ;
    rdfs:label """Has MADS Scheme
      Member"""^^xsd:string ;
    rdfs:range [
        a owl:Class ;
        owl:unionOf (madsrdf:Authority
            madsrdf:MADSCollection
        )
    ] ;
    owl:inverseOf madsrdf:isMemberOfMADSScheme .

madsrdf:hasNarrowerAuthority
    a rdf:Property, owl:ObjectProperty ;
    rdfs:comment """Creates a direct
      relationship between an Authority and one that is more narrowly defined."""^^xsd:string ;
    rdfs:label """Has Narrower
      Authority"""^^xsd:string ;
    rdfs:subPropertyOf madsrdf:hasRelatedAuthority, <http://www.w3.org/2004/02/skos/core#narrower> ;
    owl:inverseOf madsrdf:hasBroaderAuthority .

madsrdf:hasNarrowerExternalAuthority
    a rdf:Property, owl:ObjectProperty ;
    rdfs:comment """Creates a direct
      relationship between an Authority and a more narrowly defined Authority from a different MADS
      Scheme."""^^xsd:string ;
    rdfs:label """Has Narrower External
      Authority"""^^xsd:string ;
    rdfs:subPropertyOf madsrdf:hasNarrowerAuthority, <http://www.w3.org/2004/02/skos/core#narrowMatch> .

madsrdf:hasReciprocalAuthority
    a rdf:Property, owl:ObjectProperty, owl:SymmetricProperty ;
    rdfs:comment """Establishes a relationship between two Authority resources. It is
      reciprocal, so the relationship must be shared. This is Related type='equivalent' in MADS
      XML."""@en ;
    rdfs:label """Has Reciprocal
      Authority"""^^xsd:string ;
    rdfs:subPropertyOf madsrdf:hasRelatedAuthority, <http://www.w3.org/2004/02/skos/core#related> .

madsrdf:hasReciprocalExternalAuthority
    a rdf:Property, owl:ObjectProperty, owl:SymmetricProperty ;
    rdfs:comment """Establishes a relationship
      between an Authority and one from a different MADS Scheme. It is reciprocal, so the
      relationship must be shared."""^^xsd:string ;
    rdfs:label """Has Reciprocal External
      Authority"""^^xsd:string ;
    rdfs:subPropertyOf madsrdf:hasReciprocalAuthority, <http://www.w3.org/2004/02/skos/core#relatedMatch> .

madsrdf:hasRelatedAuthority
    a rdf:Property, owl:ObjectProperty ;
    rdfs:comment """Unless the relationship can be more specifically identified, use
      'hasRelatedAuthority.'"""@en ;
    rdfs:domain madsrdf:Authority ;
    rdfs:label "Has Related Authority"@en ;
    rdfs:range madsrdf:Authority ;
    rdfs:subPropertyOf <http://www.w3.org/2004/02/skos/core#semanticRelation> .

madsrdf:hasSource
    a rdf:Property, owl:ObjectProperty ;
    rdfs:comment "Associates a resource description with its Source."@en ;
    rdfs:label "Has Source"^^xsd:string ;
    rdfs:range madsrdf:Source .

madsrdf:hasTopMemberOfMADSScheme
    a rdf:Property, owl:ObjectProperty ;
    rdfs:comment """Identifies an Authority
      that is at the top of the hierarchy of authorities within the MADS Scheme."""^^xsd:string ;
    rdfs:domain madsrdf:MADSScheme ;
    rdfs:label """Has Top Member of MADS
      Scheme"""^^xsd:string ;
    rdfs:range madsrdf:Authority ;
    rdfs:subPropertyOf madsrdf:hasMADSSchemeMember, <http://www.w3.org/2004/02/skos/core#hasTopConcept> .

madsrdf:hasTranslationVariant
    a rdf:Property, owl:ObjectProperty ;
    rdfs:comment """A Variant whose label
      represents a translation of that of the authoritative label."""^^xsd:string ;
    rdfs:label """Has Translation
      Variant"""^^xsd:string ;
    rdfs:subPropertyOf madsrdf:hasVariant .

madsrdf:hasVariant
    a rdf:Property, owl:ObjectProperty ;
    rdfs:comment """Associates a Variant with an Authority or Deprecrated Authority.
      Unless the variant type can be more specifically identified, use 'hasVariant.'"""@en ;
    rdfs:domain madsrdf:Authority ;
    rdfs:label "Has Variant"^^xsd:string ;
    rdfs:range madsrdf:Variant ;
    rdfs:subPropertyOf <http://www.w3.org/2008/05/skos-xl#altLabel> .

madsrdf:hiddenLabel
    a rdf:Property, owl:DatatypeProperty ;
    rdfs:comment """A label entered for
      discovery purposes but not shown."""^^xsd:string ;
    rdfs:domain madsrdf:Variant ;
    rdfs:label "Hidden Label"^^xsd:string ;
    rdfs:subPropertyOf <http://www.w3.org/2008/05/skos-xl#literalForm> .

madsrdf:historyNote
    a owl:AnnotationProperty ;
    rdfs:comment """A note pertaining to the
      history of the resource."""^^xsd:string ;
    rdfs:label "History Note"^^xsd:string ;
    rdfs:subPropertyOf madsrdf:note ;
    owl:equivalentProperty <http://www.w3.org/2004/02/skos/core#historyNote> .

madsrdf:honoraryTitle
    a rdf:Property, owl:DatatypeProperty ;
    rdfs:comment """Designation indicative of
      royalty, nobility, or ecclesiastical rank or office, or a term of address for a person of
      religious vocation."""^^xsd:string ;
    rdfs:domain madsrdf:RWO ;
    rdfs:label "Honorary Title"^^xsd:string .

madsrdf:hours
    a rdf:Property, owl:DatatypeProperty ;
    rdfs:domain madsrdf:Affiliation ;
    rdfs:label "Hours"^^xsd:string .

madsrdf:idScheme
    a rdf:Property, owl:AnnotationProperty ;
    rdfs:comment """The scheme associated with
      the identifier. For example, \"LCCN\" would be used when the Identifier Value (madsrdf:idValue)
      is a LC Control Number."""^^xsd:string ;
    rdfs:domain madsrdf:Identifier ;
    rdfs:label """Identifier
      Scheme"""^^xsd:string .

madsrdf:idValue
    a rdf:Property, owl:DatatypeProperty ;
    rdfs:comment """The value of the identifier
      conforming to the Identifier Scheme syntax."""^^xsd:string ;
    rdfs:domain madsrdf:Identifier ;
    rdfs:label "Identifier Value"^^xsd:string ;
    rdfs:range xsd:string .

madsrdf:identifiesRWO
    a rdf:Property, owl:ObjectProperty ;
    rdfs:comment """Associates a
      madsrdf:Authority with the Real World Object that is the subject of the authority's
      label."""^^xsd:string ;
    rdfs:domain madsrdf:Authority ;
    rdfs:label "Identifies RWO"^^xsd:string ;
    rdfs:range madsrdf:RWO ;
    rdfs:subPropertyOf foaf:focus ;
    owl:inverseOf madsrdf:isIdentifiedByAuthority .

madsrdf:isIdentifiedByAuthority
    a rdf:Property, owl:ObjectProperty ;
    rdfs:comment """Associates a Real World
      Object with its Authority description."""^^xsd:string ;
    rdfs:domain madsrdf:RWO ;
    rdfs:label """Is Identified By
      Authority"""^^xsd:string ;
    rdfs:range madsrdf:Authority ;
    owl:inverseOf madsrdf:identifiesRWO .

madsrdf:isMemberOfMADSCollection
    a rdf:Property, owl:ObjectProperty ;
    rdfs:comment """Associates a Collection with a madsrdf:Authority or another
      madsrdf:MADSCollection."""@en ;
    rdfs:domain [
        a owl:Class ;
        owl:unionOf (madsrdf:Authority
            madsrdf:MADSCollection
        )
    ] ;
    rdfs:label "Is Member Of MADSCollection"@en ;
    rdfs:range madsrdf:MADSCollection ;
    owl:inverseOf madsrdf:hasMADSCollectionMember .

madsrdf:isMemberOfMADSScheme
    a rdf:Property, owl:ObjectProperty ;
    rdfs:domain [
        a owl:Class ;
        owl:unionOf (madsrdf:Authority
            madsrdf:MADSCollection
        )
    ] ;
    rdfs:label """Is Member of MADS
      Scheme"""^^xsd:string ;
    rdfs:range madsrdf:MADSScheme ;
    rdfs:subPropertyOf <http://www.w3.org/2004/02/skos/core#inScheme> ;
    owl:inverseOf madsrdf:hasMADSSchemeMember .

madsrdf:isTopMemberOfMADSScheme
    a rdf:Property, owl:ObjectProperty ;
    rdfs:comment """Identifies a MADS Scheme in
      which the Authority is at the top of the hierarchy."""^^xsd:string ;
    rdfs:domain [
        a owl:Class ;
        owl:unionOf (madsrdf:Authority
            madsrdf:MADSCollection
        )
    ] ;
    rdfs:label """Is Top Member of MADS
      Scheme"""^^xsd:string ;
    rdfs:range madsrdf:MADSScheme ;
    rdfs:subPropertyOf madsrdf:isMemberOfMADSScheme, <http://www.w3.org/2004/02/skos/core#topConceptOf> ;
    owl:inverseOf madsrdf:hasTopMemberOfMADSScheme .

madsrdf:natureOfAffiliation
    a rdf:Property, owl:AnnotationProperty ;
    rdfs:comment """Records the individual's
      role or position in the organization with which the individual is affiliated. A \"job title\"
      might be appropriate."""^^xsd:string ;
    rdfs:domain madsrdf:Affiliation ;
    rdfs:label """Nature of
      Affiliation"""^^xsd:string .

madsrdf:note
    a rdf:Property, owl:AnnotationProperty ;
    rdfs:comment """A note about the
      resource."""^^xsd:string ;
    rdfs:label "Note"^^xsd:string ;
    owl:equivalentProperty <http://www.w3.org/2004/02/skos/core#note> .

madsrdf:occupation
    a rdf:Property, owl:ObjectProperty ;
    rdfs:comment """A profession or occupation
      in which the person works or has worked."""^^xsd:string ;
    rdfs:domain madsrdf:RWO ;
    rdfs:label "Occupation"^^xsd:string ;
    rdfs:range madsrdf:Occupation .

madsrdf:organization
    a rdf:Property, owl:AnnotationProperty ;
    rdfs:comment """The group or organization
      with which an individual is associated."""^^xsd:string ;
    rdfs:domain madsrdf:Affiliation ;
    rdfs:label """Organization or
      Group"""^^xsd:string .

madsrdf:phone
    a rdf:Property, owl:DatatypeProperty ;
    rdfs:domain madsrdf:Affiliation ;
    rdfs:label "Phone"^^xsd:string .

madsrdf:postcode
    a rdf:Property, owl:DatatypeProperty ;
    rdfs:domain madsrdf:Address ;
    rdfs:label """Post Code / Zip
      Code"""^^xsd:string .

madsrdf:prominentFamilyMember
    a rdf:Property, owl:DatatypeProperty ;
    rdfs:comment """A well-known individual who
      is a member of the family."""^^xsd:string ;
    rdfs:domain madsrdf:RWO ;
    rdfs:label """Prominent Family
      Member"""^^xsd:string .

madsrdf:scopeNote
    a rdf:Property, owl:AnnotationProperty ;
    rdfs:label "Scope Note"^^xsd:string ;
    rdfs:subPropertyOf madsrdf:note ;
    owl:equivalentProperty <http://www.w3.org/2004/02/skos/core#scopeNote> .

madsrdf:see
    a owl:ObjectProperty ;
    rdfs:comment """Denotes a relationship
      between an Authority and/or DeprecatedAuthority. The relationship may or may or may not be
      reciprocated and there is no certainty that the related resource will further illuminate the
      original resource."""^^xsd:string ;
    rdfs:domain [
        a owl:Class ;
        owl:unionOf (madsrdf:Authority
            madsrdf:DeprecatedAuthority
        )
    ] ;
    rdfs:label "See Also"^^xsd:string ;
    rdfs:range [
        a owl:Class ;
        owl:unionOf (madsrdf:Authority
            madsrdf:DeprecatedAuthority
        )
    ] ;
    rdfs:subPropertyOf rdfs:seeAlso .

madsrdf:state
    a rdf:Property, owl:AnnotationProperty ;
    rdfs:comment """The state associated with
      an address."""^^xsd:string ;
    rdfs:domain madsrdf:Address ;
    rdfs:label "State"^^xsd:string .

madsrdf:streetAddress
    a rdf:Property, owl:DatatypeProperty ;
    rdfs:comment """First line of address. For
      second line, use madsrdf:extendedAddress."""^^xsd:string ;
    rdfs:domain madsrdf:Address ;
    rdfs:label "Street Address"^^xsd:string .

madsrdf:terminateDate
    a rdf:Property, owl:DatatypeProperty ;
    rdfs:comment """The year a corporate body was terminated. Date of termination may also include the month and day of the corporate body’s termination. 
    """^^xsd:string ;
    rdfs:domain madsrdf:RWO ;
    rdfs:label "Terminated"^^xsd:string .

madsrdf:useFor
    a rdf:Property, owl:ObjectProperty ;
    rdfs:comment """\"Use [This Resource] For.\"
      Traditional \"USE FOR\" reference."""^^xsd:string ;
    rdfs:label "Use For"^^xsd:string ;
    rdfs:subPropertyOf madsrdf:see ;
    owl:inverseOf madsrdf:useInstead .

madsrdf:useInstead
    a rdf:Property, owl:ObjectProperty ;
    rdfs:comment """\"Use [This Other Resource]
      Instead.\" Traditional \"USE\" reference."""^^xsd:string ;
    rdfs:label "Use Instead"^^xsd:string ;
    rdfs:subPropertyOf madsrdf:see .

madsrdf:variantLabel
    a rdf:Property, owl:DatatypeProperty ;
    rdfs:comment """The lexical, variant form
      of an authoritative label."""^^xsd:string ;
    rdfs:domain madsrdf:Variant ;
    rdfs:label "Variant Label"^^xsd:string ;
    rdfs:subPropertyOf <http://www.w3.org/2008/05/skos-xl#literalForm> .

madsrdf:workOrigin
    a rdf:Property, owl:ObjectProperty ;
    rdfs:comment "The country or other territorial jurisdiction from which a work originated."^^xsd:string ;
    rdfs:label "Work locale"^^xsd:string ;
    rdfs:range madsrdf:Geographic .

<http://www.loc.gov/standards/mads/rdf/v1.rdf>
    a owl:Ontology ;
    rdfs:comment """Updated: 10 May 2012 - Added Language Class; componentList and
      elementList now has the union of rdf:List or rdf:Seq for a range."""@en .

rdfs:comment
    a owl:AnnotationProperty .

rdfs:label
    a owl:AnnotationProperty .

xsd:date
    a rdfs:Datatype .

owl:Thing
    a owl:Class .

